# Problem 1 (solution)

> [!NOTE]
> Constants of integration are manipulated rather liberally, without assigning new indices, often absorb other constants implicitly. Usually they will be denoted as $C_n$

Solve for $u(x, t)$

$$
\begin{cases}
\frac{\partial u}{\partial t}=\alpha\frac{\partial^2u}{\partial x^2}\\
u(x,0)=0\\
u(0,t)=T_1\\
u(1,t)=T_2
\end{cases}
$$ 

## Deal with boundary conditions

### An idea

We cannot yet assume separation of variables because boundary conditions are not homogenous.

To deal with this we can think about this problem from another angle. The rod edges will always stay the same temperature. This means that eventually the temperature along the rod will reach an equilibrium.

$$\lim_{t\to\infty}{u(x,t)}=u_E(x)$$

This solution should also satisfy the problem so

$$\partial_t u_E=\alpha\partial_{xx}u_E$$

but $u_E$ only depends on $x$ so $\partial_t u_E=0$

$$
\begin{align}
\frac{d^2u_E}{dx^2}&=0\\
d^2u_E&=0dx^2\\
\int d(du_E)&=\int 0dx^2\\
du_E&=C_1dx\\
\int du_E&=\int C_1dx\\
u_E&=C_1x+C_2
\end{align}
$$

Initial conditions also must hold

$$
\begin{cases}
u_E(0)=T_1\Rightarrow C_2=T_1\\
u_E(1)=T_2\Rightarrow C_1+T_1=T_2\Rightarrow C1=T_2-T_1
\end{cases}
$$

Finally $u_E(x)=(T_2-T_1)x+T_1=T_2x+T_1(1-x)$

### The point

We can now define a function $v(x,t)=u(x,t)-u_E(x,t)$ and rewrite it as $u(x,t)=v(x,t)+u_E(x,t)$. Now because $u_E$ is independent of time and is only a first degree polynomial, it holds that

$$
\begin{align}
\partial_t u=\partial_t v+\partial_t u_E&=\partial_t v\\
\partial_{xx}u=\partial_{xx}v+\partial_{xx}u_E&=\partial_{xx}v 
\end{align}
$$

This means that $u$ and $v$ will satisfy the same PDE. However, the boundary conditions change for $v$

$$
\begin{cases}
v(x,0)=u(x,0)-u_E(x)=(T_1-T_2)x-T_1\\
v(0,t)=u(0,t)-u_E(0)=T_1-T_1=0\\
v(1,t)=u(1,t)-u_E(1)=T_2-T_2=0
\end{cases}
$$

We now have homogenous boundary conditions (even though the initial condition is messier)

## Separation of variables

Assume $v(x,t)=\varphi(x)G(t)$, then the PDE becomes

$$ 
\begin{align}
\varphi(x)\dot G(t)=\alpha\varphi''(x)G(t)\\
\frac{1}{\alpha G}\frac{dG}{dt}=\frac{1}{\varphi}\frac{d^2\varphi}{dx^2}=-\lambda
\end{align}
$$

$-\lambda$ here is the separation constant. This yields a new system.

$$
\begin{cases}
\frac{dG}{dt}=-\alpha\lambda G\\
\frac{d^2\varphi}{dx^2}=-\lambda\varphi
\end{cases}
$$

First equation is trivial to solve: $G(t)=C_1e^{-\alpha\lambda t}$.

## Getting rid of trivial solutions

The boundary conditions must hold for $v$, so 

$$ 
\begin{cases}
v(0,t)=0\Rightarrow\varphi(0)G(t)=0\\
v(1,t)=0\Rightarrow\varphi(1)G(t)=0
\end{cases}
$$

In the first equation, either $\varphi(0)=0$ or $G(t)=0$, but if $G(t)=0$ then $v(x,t)=0$. This is a trivial solution and does not interest us, so we assume $\varphi(0)=0$. The second equations hold the same problem so we must assume $\varphi(1)=0$. We now have a system

$$
\begin{cases}
\frac{d^2\varphi}{dx^2}=-\lambda\varphi\\
\varphi(0)=0\\
\varphi(1)=0
\end{cases}
$$

## Solving the spacial equation

Second eq. prerequisites. 

Let $\theta=\frac{d\varphi}{dx}$, then $dx=\frac{d\varphi}{\theta}$ and $\theta'=\frac{d\theta}{dx}=\theta\frac{d\theta}{d\varphi}$

Second eq.

$$
\begin{align}
\theta\frac{d\theta}{d\varphi}&=-\lambda\varphi\\
\int\theta d\theta&=-\lambda\int\varphi d\varphi\\
\frac{\theta^2}{2}&=-\lambda\frac{\varphi^2}{2}+C_1\\
\theta^2&=C_1-\lambda\varphi^2\\
\theta&=\sqrt{C_1-\lambda\varphi^2}\\
\frac{d\varphi}{dx}&=\sqrt{C_1-\lambda\varphi^2}\\
\int\frac{d\varphi}{\sqrt{C_1-\lambda\varphi^2}}&=x+C_2
\end{align}
$$

We now split our problem into three distict cases

### Case where $\lambda = 0$

In this case the equation becomes

$$
C_1\int d\varphi=x+C_2\Rightarrow C_1\varphi=x+C_2\Rightarrow \varphi(x)=C_1x+C_2
$$

Boundary conditions

$$
\begin{cases}
\varphi(0)=0\Rightarrow C_2=0\\
\varphi(1)=0\Rightarrow C_1=0
\end{cases}
$$

This gets us the trivial solution in which, again, we are not interested.

### Case where $\lambda < 0$


$$
\begin{align}
\int\frac{d\varphi}{\sqrt{C_1-\lambda\varphi^2}}&=x+C_2\\
\frac{1}{\sqrt{-\lambda}}\int\frac{d(\sqrt{-\lambda}\varphi)}{\sqrt{C_1+(\sqrt{-\lambda}\varphi)^2}}&=x+C_2\\
\frac{1}{\sqrt{-\lambda}}ln\left|\sqrt{-\lambda}\varphi+\sqrt{-\lambda\varphi^2+C_1}\right|&=x+C_2\\ 
ln\left|\sqrt{-\lambda}\varphi+\sqrt{-\lambda\varphi^2+C_1} \right|&=\sqrt{-\lambda}x+C_2\\
\sqrt{-\lambda}\varphi+\sqrt{-\lambda\varphi^2+C_1}&=C_2e^{\sqrt{-\lambda}x}\\ 
\varphi+\sqrt{\varphi^2+C_1}&=C_2e^{\sqrt{-\lambda}x}\\
\sqrt{\varphi^2+C_1}&=C_2e^{\sqrt{-\lambda}x}-\varphi\\
\varphi^2+C_1&=C_2^2e^{2\sqrt{-\lambda}x}-2C_2e^{\sqrt{-\lambda}x}\varphi+\varphi^2\\
C_1&=C_2^2e^{2\sqrt{-\lambda}x}-2C_2e^{\sqrt{-\lambda}x}\varphi\\
2C_2e^{\sqrt{-\lambda}x}\varphi&=C_2^2e^{2\sqrt{-\lambda}x}-C_1\\
\varphi&=\frac{C_2^2e^{2\sqrt{-\lambda}x}-C_1}{2C_2e^{\sqrt{-\lambda}x}}\\
\varphi&=\frac{1}{2}\left[\frac{C_2^2e^{2\sqrt{-\lambda}x}}{C_2e^{\sqrt{-\lambda}x}}-\frac{C_1}{C_2e^{\sqrt{-\lambda}x}} \right]\\
\varphi&=\frac{1}{2}\left[C_2e^{\sqrt{-\lambda}x}-C_1e^{-\sqrt{-\lambda}x}\right]\\
\varphi&=\frac{1}{2}\left[C_1e^{\sqrt{-\lambda}x}+C_2e^{\sqrt{-\lambda}x}+C_1e^{-\sqrt{-\lambda}x}-C_2e^{-\sqrt{-\lambda}x}\right]\\
\varphi(x)&=C_1\cosh(\sqrt{-\lambda}x)+C_2\sinh(\sqrt{-\lambda}x)
\end{align}
$$

Now we need to check for boundary conditions to determine constants.

$$\varphi(0)=C_1\cosh(0)+C_2\sinh(0)=C_1=0$$

Now because $C_1=0$

$$\varphi(1)=C_2\sinh(\sqrt{-\lambda})$$

but $\sqrt{-\lambda}\ne 0$, so $\sinh(\sqrt{-\lambda})\ne 0$, but we cannot have that because it would yield a trivial solution as $C_1=0$ and $C_2=0$.

### Case where $\lambda>0$

$$
\begin{align}
\int\frac{d\varphi}{\sqrt{C_1-\lambda\varphi^2}}&=x+C_2\\
\frac{1}{\sqrt{\lambda}}\int\frac{d(\sqrt{\lambda}\varphi)}{\sqrt{C_1-(\sqrt{\lambda}\varphi)^2}}&=x+C_2\\
\frac{1}{\sqrt{\lambda}}\int\frac{d(\sqrt{\lambda}\varphi)}{\sqrt{C_1-(\sqrt{\lambda}\varphi)^2}}&=x+C_2\\
\frac{1}{\sqrt{\lambda}}\arcsin\left(\frac{\sqrt{\lambda}\varphi}{C_1}\right)&=x+C_2\\
\arcsin\left(\frac{\sqrt{\lambda}\varphi}{C_1}\right)&=\sqrt{\lambda}x+C_2\\
\frac{\sqrt{\lambda}\varphi}{C_1}&=\sin\left(\sqrt{\lambda}x+C_2\right)\\
\varphi&=C_1\sin\left(\sqrt{\lambda}x+C_2\right)\\
\varphi&=C_1\sin\left(\sqrt{\lambda}x\right)\cos(C_2)+C_1\cos\left(\sqrt{\lambda}x\right)\sin(C_2)\\
\varphi&=C_1\sin\left(\sqrt{\lambda}x\right)+C_2\cos\left(\sqrt{\lambda}x\right)
\end{align}
$$

First boundary condition

$$
\varphi(0)=C_2\cos\sqrt\lambda\Rightarrow C_2=0
$$

using the last result

$$
\varphi(1)=C_1\sin(\sqrt\lambda)=0
$$

$C_1=0$ would bring us back to the trivial solution, so $\sin(\sqrt\lambda)=0$ and $\lambda_n=(\pi n)^2,n\in\N$. Note that this gives us infinite solutions because of the superposition principle.

## Putting it all together

The final solution will have the form

$$
v(x,t)=\sum_{n=1}^{\infty}B_ne^{-\alpha(\pi n)^2t}\sin(\pi n x)
$$

This solution has to satisfy the initial condition so

$$
v(x,0)=\sum_{n=1}^{\infty}B_n\sin(\pi n x)=(T_1-T_2)x-T_1
$$

We can notice that at the initial condition the solution coefficients $B_n$ are Fourier sine series coefficients and so can be easily calculated using the formula below
$$
B_n=\frac{2}{L}\int_{0}^{L}v(x,0)\sin\left(\frac{2\pi nx}{L}\right)dx
$$

We will take $L=1$

$$
\begin{align}
B_n&=2\int_{0}^{1}((T_1-T_2)x-T_1)\sin\left(2 \pi nx\right)dx\\
B_n&=2\int_{0}^{1}(T_1-T_2)x\sin\left(2 \pi nx\right)dx-2\int_{0}^{1}T_1\sin\left(2 \pi nx\right)dx
\end{align}
$$

First let's evaluate the first integral

$$
\begin{align}
\int_{0}^{1}(T_1-T_2)x\sin\left(2 \pi nx\right)dx\\
-\frac{T_1-T_2}{2\pi n}\int_{0}^{1}xd\cos(2\pi nx)\\
-\frac{T_1-T_2}{2\pi n}\left(x\cos(2\pi nx)\bigg\rvert_{0}^{1}-\int_{0}^{1}\cos(2\pi nx)dx\right)\\
-\frac{T_1-T_2}{2\pi n}\left(1-\frac{\sin(2\pi nx)}{2\pi n}\bigg\rvert_{0}^{1}\right)\\
-\frac{T_1-T_2}{2\pi n}
\end{align}
$$

Now for the second integral

$$
\begin{align}
\int_{0}^{1}T_1\sin\left(2 \pi nx\right)dx\\
-T_1\frac{\cos(2\pi nx)}{2\pi n}\bigg\rvert_{0}^{1}\\
-T_1\left(\frac{1}{2\pi n}-\frac{1}{2\pi n}\right)\\
0
\end{align}
$$

Finally

$$
B_n=-2\frac{T_1-T_2}{2\pi n} = \frac{T_2-T_1}{\pi n}
$$

and

$$
v(x,t)=\sum_{n=1}^{\infty}\frac{T_2-T_1}{\pi n}e^{-\alpha(\pi n)^2t}\sin(\pi n x)
$$